formalization/Reduction.v
@@ -27,3 +27,46 @@ Inductive reduces : process -> process -> Prop :=
                 P ≡ P' -> P' ⊳ Q' -> Q' ≡ Q -> P ⊳ Q
 where
   "P ⊳ Q" := (reduces P Q).
+
+(******************************************************************************)
+(* Reduction (depth-indexed)                                                  *)
+(******************************************************************************)
+Inductive reduces_d : nat -> process -> process -> Prop :=
+  | r_tensor_par_d : forall P Q R P',
+                      P' = rename_process (up P) swap01 ->
+                      reduces_d 0
+                        (link (prefix (send P Q)) (prefix (receive R)))
+                        (cut (cut R P') Q)
+  | r_plus_with_l_d : forall P Q R,
+                        reduces_d 0
+                          (link (prefix (choose_left P)) (prefix (offer_choice Q R)))
+                          (cut P Q)
+  | r_plus_with_r_d : forall P Q R,
+                        reduces_d 0
+                          (link (prefix (choose_right P)) (prefix (offer_choice Q R)))
+                          (cut P R)
+  | r_one_bot_d : forall P, reduces_d 0 (link (prefix close) (prefix (wait P))) P
+  | r_ax_cut_d : forall M P,
+                  reduces_d 0
+                    (cut (link (future 0) M) P)
+                    (subst_process P ((downM M) ⋅ id_subst))
+  | r_seq_d : forall P s, reduces_d 0 (seq P s) (subst_process P ((prefix s) ⋅ id_subst))
+  | r_cong_cut_d : forall P P' Q n,
+                    reduces_d n P P' ->
+                    reduces_d (S n) (cut P Q) (cut P' Q)
+  | r_cong_seq_d : forall P P' s n,
+                    reduces_d n P P' -> reduces_d (S n) (seq P s) (seq P' s)
+  | r_struct_d : forall P P' Q Q' n,
+                  P ≡ P' -> reduces_d n P' Q' -> Q' ≡ Q -> reduces_d (S n) P Q.
+
+Lemma reduces_d_from_reduces :
+  forall P P', P ⊳ P' -> exists k, reduces_d k P P'.
+Proof.
+  apply reduces_ind; intros;
+    try (now (exists 0; econstructor; eauto));
+    try destruct H0; try destruct H1; exists (S x); econstructor; eauto.
+Qed.
+
+Lemma reduces_from_reduces_d :
+  forall k P Q, reduces_d k P Q -> P ⊳ Q.
+Proof. intros. induction H; econstructor; eauto. Qed.
