formalization/Irreducibility.v
@@ -1,0 +1,390 @@
+From FD Require Import Syntax.
+From FD Require Import Types.
+From FD Require Import StructCong.
+From FD Require Import Reduction.
+From FD Require Import Contexts.
+From FD Require Import Typing.
+From FD Require Import FinalProcess.
+From FD Require Import Progress.
+
+From Stdlib Require List.
+From Stdlib Require Import PeanoNat.
+From Stdlib Require Import Lia.
+Import List.ListNotations.
+
+(******************************************************************************)
+(* Irreducibility                                                             *)
+(******************************************************************************)
+Definition irreducible P := forall Q, ~ (P ⊳ Q).
+
+(******************************************************************************)
+(* The notion of final process coindices with irreducibility                  *)
+(******************************************************************************)
+(* We want to show, that for every well-typed P, final P iff irreducible P *)
+(* The direction <- follows immediately by progress  *)
+Lemma irreducible_implies_final :
+  forall Γ P, Γ ⊢ P :# -> irreducible P -> final P.
+Proof.
+  intros. apply progress in H. destruct H as [[P' ?] |]; auto.
+  exfalso. apply (H0 P'); auto.
+Qed.
+
+(* For the direction -> we require additional lemmata *)
+(* Stop is irreducible *)
+Lemma stop_irreducible : forall P, P = stop -> irreducible P.
+Proof.
+  intros P Hstop Q Hred.
+  induction Hred; try discriminate; subst.
+  apply IHHred.
+  apply stop_equiv_stop; auto.
+Qed.
+
+(* Links containing futures are irreducible *)
+Lemma link_future_irreducible_d :
+    forall n,
+      forall k i M P,
+        k <= n ->
+        P ≡ (link (future i) M) ->
+        forall Q, ~ (reduces_d k P Q).
+Proof.
+  induction n; intros; intro Hred.
+  + assert (k = 0) by lia; subst. inversion Hred; subst; try congruence;
+    try match goal with
+    | [ H : _ ≡ _ |- _ ] =>
+        destruct (link_future_equiv_link_future _ _ _ (or_intror H)) as [M' [n' [? [? | ?]]]];
+        try congruence
+    end.
+  + inversion Hred; subst;
+    try match goal with
+    | [ H : _ ≡ _ |- _ ] =>
+        destruct (link_future_equiv_link_future _ _ _ (or_intror H)) as [M' [n' [? [? | ?]]]];
+        try congruence
+    end.
+    - assert (n0 <= n) by lia.
+      assert (P' ≡ (link (future i) M)). { eapply c_trans; eauto. apply c_comm; auto. }
+      apply (IHn _ _ _ _ H6 H7 Q'); auto.
+    - assert (n0 <= n) by lia.
+      assert (P' ≡ (link (future i) M)). { eapply c_trans; eauto. apply c_comm; auto. }
+      apply (IHn _ _ _ _ H6 H7 Q'); auto.
+Qed.
+
+Lemma link_future_irreducible :
+  forall i M P,
+    P ≡ (link (future i) M) ->
+    irreducible P.
+Proof.
+  intros. intros Q Hred.
+  apply reduces_d_from_reduces in Hred. destruct Hred.
+  eapply link_future_irreducible_d in H0; auto.
+  apply H.
+Qed.
+
+(* Link trees are irreducible *)
+Inductive link_tree : nat -> process -> Prop :=
+  | link_tree_leaf_nn : forall i i1 i2 M1 M2 P1 P2,
+                    no_future M1 -> no_future M2 ->
+                    i < i1 -> i < i2 ->
+                    P1 ≡ (link (future i1) M1) ->
+                    P2 ≡ (link (future i2) M2) ->
+                    link_tree i (cut P1 P2)
+  | link_tree_leaf_nf : forall i i1 i2 i3 M P,
+                    no_future M ->
+                    i < i1 -> i < i2 -> i < i3 ->
+                    P ≡ (link (future i3) M) ->
+                    link_tree i (cut (link (future i1) (future i2)) P)
+  | link_tree_leaf_fn : forall i i1 i2 i3 M P,
+                          no_future M ->
+                          i < i1 -> i < i2 -> i < i3 ->
+                          P ≡ (link (future i1) M) ->
+                          link_tree i (cut P (link (future i2) (future i3)))
+  | link_tree_leaf_ff : forall i i1 i2 i3 i4,
+                          i < i1 -> i < i2 -> i < i3 -> i < i4 ->
+                          link_tree i
+                            (cut (link (future i1) (future i2)) (link (future i3) (future i4)))
+  | link_tree_cons_nl : forall i i' M P L,
+                          link_tree (S i) P ->
+                          no_future M ->
+                          i < i' ->
+                          L ≡ (link (future i') M) ->
+                          link_tree i (cut L P)
+  | link_tree_cons_nr : forall i i' M P R,
+                          link_tree (S i) P ->
+                          no_future M ->
+                          i < i' ->
+                          R ≡ (link (future i') M) ->
+                          link_tree i (cut P R)
+  | link_tree_cons_fl : forall i i1 i2 P,
+                          link_tree (S i) P ->
+                          i < i1 -> i < i2 ->
+                          link_tree i (cut (link (future i1) (future i2)) P)
+  | link_tree_cons_fr : forall i i1 i2 P,
+                          link_tree (S i) P ->
+                          i < i1 -> i < i2 ->
+                          link_tree i (cut P (link (future i1) (future i2)))
+  | link_tree_branch : forall i P Q,
+                        link_tree (S i) P -> link_tree (S i) Q -> link_tree i (cut P Q).
+
+(* A final link list is a link tree *)
+Lemma final_link_list_is_link_tree' :
+  forall j xs P,
+    (forall x, List.In x xs -> x > j) -> link_list xs P -> link_tree j P.
+Proof.
+  intros.
+  generalize dependent j.
+  induction H0; intros.
+  + destruct M1, M2; try congruence.
+    destruct (link_future_equiv_link_future _ _ _ (or_intror H1)) as [? [? [? ?]]].
+    destruct (link_future_equiv_link_future _ _ _ (or_intror H2)) as [? [? [? ?]]].
+    destruct H5, H7; subst; simpl in H3.
+    - destruct x, x1; try now inversion H4.
+      eapply link_tree_leaf_nn; try apply c_refl; try congruence;
+      [ specialize H3 with i1 | specialize H3 with i2 ]; lia.
+    - destruct x, x1; try now inversion H4.
+      eapply link_tree_leaf_nn; try apply c_refl; try apply c_link; try congruence;
+      [ specialize H3 with i1 | specialize H3 with i2 ]; lia.
+    - destruct x, x1; try now inversion H4.
+      eapply link_tree_leaf_nn; try apply c_refl; try apply c_link; try congruence;
+      [ specialize H3 with i1 | specialize H3 with i2 ]; lia.
+    - destruct x, x1; try now inversion H4.
+      eapply link_tree_leaf_nn; try apply c_refl; try apply c_link; try congruence;
+      [ specialize H3 with i1 | specialize H3 with i2 ]; lia.
+  + destruct M; try congruence.
+    destruct (link_future_equiv_link_future _ _ _ (or_intror H0)) as [? [? [? ?]]].
+    destruct x. inversion H2. simpl in H1.
+    destruct H3; subst.
+    - eapply link_tree_leaf_nf; try apply c_refl; try congruence;
+      [ specialize H1 with i1 | specialize H1 with i2 | specialize H1 with i3 ]; lia.
+    - eapply link_tree_leaf_nf; try apply c_link; try congruence;
+      [ specialize H1 with i1 | specialize H1 with i2 | specialize H1 with i3 ]; lia.
+  + destruct M; try congruence.
+    destruct (link_future_equiv_link_future _ _ _ (or_intror H0)) as [? [? [? ?]]].
+    destruct x. inversion H2. simpl in H1.
+    destruct H3; subst.
+    - eapply link_tree_leaf_fn; try apply c_refl; try congruence;
+      [ specialize H1 with i1 | specialize H1 with i2 | specialize H1 with i3 ]; lia.
+    - eapply link_tree_leaf_fn; try apply c_link; try congruence;
+      [ specialize H1 with i1 | specialize H1 with i2 | specialize H1 with i3 ]; lia.
+  + apply link_tree_leaf_ff; simpl in H;
+    [ specialize H with i1 | specialize H with i2 | specialize H with i3 | specialize H with i4 ]; lia.
+  + pose proof (H2 i). simpl in H3.
+    eapply link_tree_cons_nl.
+    * apply IHlink_list; intros. apply List.in_map_iff in H4. destruct H4 as [x' [? ?]].
+      subst. specialize H2 with x'. simpl in H2. pose proof (H2 (or_intror H5)). lia.
+    * eassumption.
+    * eapply H2. simpl. left. reflexivity.
+    * eassumption.
+  + pose proof (H i1). simpl in H1.
+    pose proof (H i2). simpl in H2.
+    simpl in H.
+    eapply link_tree_cons_fl.
+    * apply IHlink_list; intros. apply List.in_map_iff in H3. destruct H3 as [x' [? ?]].
+      subst. specialize H with x'. pose proof (H (or_intror (or_intror H4))). lia.
+    * lia.
+    * lia.
+Qed.
+
+Lemma final_link_list_is_link_tree :
+  forall xs P,
+    ~ (List.In 0 xs) -> link_list xs P -> link_tree 0 P.
+Proof.
+  intros. eapply final_link_list_is_link_tree'; eauto.
+  intros. destruct x; [congruence | lia].
+Qed.
+
+(* Link treenes is preserved under structural congruence *)
+Lemma struct_cong_preserves_link_tree' :
+  forall n,
+    forall k,
+      k <= n ->
+        forall j P Q,
+          link_tree j P ->
+          (struct_cong_d k P Q) \/ (struct_cong_d k Q P) ->
+          link_tree j Q.
+Proof.
+  (* induction n; intros.
+  + assert (k = 0) by lia; subst. destruct H1; inversion H1; subst.
+    - inversion H0.
+    - inversion H0; subst; econstructor; eauto.
+    - inversion H0; subst.
+      * inversion H7; subst; simpl; econstructor; admit.
+      * inversion H7; subst; simpl; econstructor; admit.
+      * inversion H6; subst; admit.
+    - auto.
+    - inversion H0.
+    - inversion H0; subst; econstructor; eauto.
+    - inversion H0; subst.
+      * destruct P0; simpl in H3; try congruence.
+        inversion H3; subst.
+        admit.
+      * admit.
+      * admit.
+    - auto.
+  + destruct H1.
+    - inversion H1; subst.
+      * inversion H0.
+      * inversion H0; subst; econstructor; eauto.
+      * admit.
+      * auto.
+      * eapply (IHn n0); eauto. lia.
+      * assert (link_tree j Q0). { eapply (IHn n1); eauto. lia. }
+        eapply (IHn n2); eauto. lia.
+      * inversion H0.
+      * inversion H0; subst.
+        ** admit.
+        ** admit.
+        ** admit.
+        ** admit.
+        ** admit.
+        ** admit.
+        ** admit.
+        ** admit.
+        ** admit.
+      * inversion H0.
+    - inversion H1; subst.
+      * inversion H0.
+      * inversion H0; subst; econstructor; eauto.
+      * admit.
+      * auto.
+      * eapply (IHn n0); eauto. lia.
+      * assert (link_tree j Q0). { eapply (IHn n2); eauto. lia. }
+        eapply (IHn n1); eauto. lia.
+      * inversion H0.
+      * admit.
+      * inversion H0. *)
+Admitted.
+
+Lemma struct_cong_preserves_link_tree :
+  forall j P Q, link_tree j P -> P ≡ Q -> link_tree j Q.
+Proof.
+  intros.
+  eapply (proj1 struct_cong_d_from_struct_cong) in H0. destruct H0.
+  eapply struct_cong_preserves_link_tree'; eauto.
+Qed.
+
+Lemma link_tree_irreducible' :
+  forall n,
+    forall k,
+      k <= n ->
+      forall j P, link_tree j P -> (forall Q, ~ (reduces_d k P Q)).
+Proof.
+  induction n; intros; intro Hred.
+  + assert (k = 0) by lia; subst. inversion Hred; subst; try now inversion H0.
+    inversion H0; subst; exfalso; try lia.
+    - destruct (link_future_equiv_link_future _ _ _ (or_introl H8)) as [? [? [? [? | ?]]]].
+      * inversion H2; subst. lia.
+      * inversion H2; subst. congruence.
+    - destruct (link_future_equiv_link_future _ _ _ (or_introl H8)) as [? [? [? [? | ?]]]].
+      * inversion H2; subst. lia.
+      * inversion H2; subst. congruence.
+    - destruct (link_future_equiv_link_future _ _ _ (or_introl H7)) as [? [? [? [? | ?]]]].
+      * inversion H2; subst. lia.
+      * inversion H2; subst. congruence.
+    - inversion H3.
+    - inversion H3.
+    - inversion H4.
+  + inversion H0; subst.
+    - inversion Hred; subst.
+      * destruct (link_future_equiv_link_future _ _ _ (or_introl H5)) as [? [? [? [? | ?]]]].
+        ** inversion H8; subst. lia.
+        ** inversion H8; subst. congruence.
+      * apply (link_future_irreducible _ _ _ H5 P').
+        apply reduces_from_reduces_d in H11; auto.
+      * assert (n0 <= n) by lia.
+        apply (struct_cong_preserves_link_tree _ _ _ H0) in H7.
+        apply (IHn n0 H10 _ _ H7 Q'); auto.
+    - inversion Hred; subst.
+      * inversion H0; lia.
+      * assert ((link (future i1) (future i2)) ≡ (link (future i1) (future i2))) by apply c_refl.
+        apply (link_future_irreducible _ _ _ H6 P').
+        apply reduces_from_reduces_d in H10; auto.
+      * assert (n0 <= n) by lia.
+        apply (struct_cong_preserves_link_tree _ _ _ H0) in H6.
+        apply (IHn n0 H9 _ _ H6 Q'); auto.
+    - inversion Hred; subst.
+      * destruct (link_future_equiv_link_future _ _ _ (or_introl H5)) as [? [? [? [? | ?]]]].
+        ** inversion H7; subst. lia.
+        ** inversion H7; subst. congruence.
+      * apply (link_future_irreducible _ _ _ H5 P').
+        apply reduces_from_reduces_d in H10; auto.
+      * assert (n0 <= n) by lia.
+        apply (struct_cong_preserves_link_tree _ _ _ H0) in H6.
+        apply (IHn n0 H9 _ _ H6 Q'); auto.
+    - inversion Hred; subst.
+      * lia.
+      * assert ((link (future i1) (future i2)) ≡ (link (future i1) (future i2))) by apply c_refl.
+        apply (link_future_irreducible _ _ _ H5 P').
+        apply reduces_from_reduces_d in H9; auto.
+      * assert (n0 <= n) by lia.
+        apply (struct_cong_preserves_link_tree _ _ _ H0) in H5.
+        apply (IHn n0 H8 _ _ H5 Q'); auto.
+    - inversion Hred; subst.
+      * destruct (link_future_equiv_link_future _ _ _ (or_introl H4)) as [? [? [? [? | ?]]]].
+        ** inversion H6; subst. lia.
+        ** inversion H6; subst. congruence.
+      * apply (link_future_irreducible _ _ _ H4 P').
+        apply reduces_from_reduces_d in H9; auto.
+      * assert (n0 <= n) by lia.
+        apply (struct_cong_preserves_link_tree _ _ _ H0) in H5.
+        apply (IHn n0 H8 _ _ H5 Q'); auto.
+    - inversion Hred; subst.
+      * inversion H1.
+      * assert (n0 <= n) by lia.
+        apply (IHn n0 H5 _ _ H1 P'); auto.
+      * assert (n0 <= n) by lia.
+        apply (struct_cong_preserves_link_tree _ _ _ H0) in H5.
+        apply (IHn n0 H8 _ _ H5 Q'); auto.
+    - inversion Hred; subst.
+      * lia.
+      * assert ((link (future i1) (future i2)) ≡ (link (future i1) (future i2))) by apply c_refl.
+        apply (link_future_irreducible _ _ _ H4 P').
+        apply reduces_from_reduces_d in H8; auto.
+      * assert (n0 <= n) by lia.
+        apply (struct_cong_preserves_link_tree _ _ _ H0) in H4.
+        apply (IHn n0 H7 _ _ H4 Q'); auto.
+    - inversion Hred; subst.
+      * inversion H1.
+      * assert (n0 <= n) by lia.
+        apply (IHn n0 H4 _ _ H1 P'); auto.
+      * assert (n0 <= n) by lia.
+        apply (struct_cong_preserves_link_tree _ _ _ H0) in H4.
+        apply (IHn n0 H7 _ _ H4 Q'); auto.
+    - inversion Hred; subst.
+      * inversion H1.
+      * assert (n0 <= n) by lia.
+        apply (IHn n0 H3 _ _ H1 P'); auto.
+      * assert (n0 <= n) by lia.
+        apply (struct_cong_preserves_link_tree _ _ _ H0) in H3.
+        apply (IHn n0 H6 _ _ H3 Q'); auto.
+Qed.
+
+Lemma link_tree_irreducible :
+  forall j P, link_tree j P -> irreducible P.
+Proof.
+  intros. intros Q Hred. apply reduces_d_from_reduces in Hred. destruct Hred.
+  eapply link_tree_irreducible' in H0; eauto.
+Qed.
+
+(* The direction -> uses the facts above:
+   stop, links with futures and link trees are irreducible *)
+Lemma final_implies_irreducible :
+  forall Γ P, Γ ⊢ P :# -> final P -> irreducible P.
+Proof.
+  intros. inversion H0.
+  + apply stop_irreducible. reflexivity.
+  + eapply link_future_irreducible. apply c_refl.
+  + eapply link_future_irreducible. apply c_link.
+  + assert (link_tree 0 P'). { apply (final_link_list_is_link_tree _ _ H1 H2). }
+    (* link_treenes is preserved under structural congruence *)
+    apply c_comm in H3.
+    pose proof (struct_cong_preserves_link_tree _ _ _ H5 H3).
+    (* link_trees are irreducible *)
+    eapply link_tree_irreducible; eauto.
+Qed.
+
+Corollary final_iff_irreducible :
+  forall Γ P, Γ ⊢ P :# -> final P <-> irreducible P.
+Proof.
+  intros; split.
+  + eapply final_implies_irreducible; eauto.
+  + eapply irreducible_implies_final; eauto.
+Qed.
